

Derivation of $r(\pi^T, d^{p-2})$ on (3)

Derivation using $E(E(L(u, d(X))|u))$:

$$d^{p-2} = \left(1 - \frac{p-2}{\|X\|^2}\right)X$$

$$R(u, d^{p-2}(X)) = E_X(\|u - \left(1 - \frac{p-2}{\|X\|^2}\right)X\|^2 | u)$$

By previous class

$$= p - (p-2)^2 E\left(\frac{1}{\|X\|^2} | u\right)$$

$$r(\pi^T, d^{p-2}(X)) = E_u[R(u, d^{p-2}(X))]$$

$$= E_u\left(p - (p-2)^2 E_{X|u}\left(\frac{1}{\|X\|^2} | u\right)\right)$$

$$= p - (p-2)^2 \cdot E_X\left(\frac{1}{\|X\|^2}\right)$$

$$= p - (p-2)^2 \cdot \frac{1}{(p-2)(\tau^2+1)}$$

$$= p - \frac{p-2}{(\tau^2+1)}$$

$$= \frac{p\tau^2 + 2}{\tau^2 + 1}$$

Another derivation using $E(E(L(u, d(X))|X)$

$$d_i = \left(1 - \frac{p-2}{\|X\|^2}\right) X_i$$

$$u_i | X_i \sim N\left(\frac{\tau^2}{1+\tau^2} X_i, \frac{\tau^2}{1+\tau^2}\right)$$

$$X_i \sim N(0, 1 + \tau_i^2)$$

$$E((u_i - d_i)^2 | X_i)$$

$$= \text{Var}(u_i | X_i) + (E(u_i | X_i) - d_i)^2$$

$$= \frac{\tau^2}{1+\tau^2} + \left(\frac{\tau^2}{1+\tau^2} X_i - \left(1 - \frac{p-2}{\|X\|^2}\right) X_i\right)^2$$

$$= \frac{\tau^2}{1+\tau^2} + \left(\frac{\tau^2}{1+\tau^2} - 1 + \frac{p-2}{\|X\|^2}\right)^2 X_i^2$$

$$= \frac{\tau^2}{1+\tau^2} + \left(\frac{p-2}{\|X\|^2} - \frac{1}{1+\tau^2}\right)^2 X_i^2$$

$$\sum_{i=1}^p E((u_i - d_i)^2 | X_i)$$

$$= \frac{p \tau^2}{1+\tau^2} + \left(\frac{p-2}{\|X\|^2} - \frac{1}{1+\tau^2}\right)^2 \cdot \|X\|^2$$

$$= \frac{p \tau^2}{1+\tau^2} + \frac{(p-2)^2}{\|X\|^2} - \frac{2(p-2)}{1+\tau^2} + \frac{\|X\|^2}{(1+\tau^2)^2}$$

$$E \left(\frac{\|X\|^2}{1+\tau^2} \right)$$

$$E \|X\|^2 = (1+\tau^2) p, \text{ Since } X_i/\sqrt{1+\tau^2} \sim N(0,1)$$

$$E(1/\|X\|^2) = 1/[(p-2)(1+\tau^2)]$$

$$E \left(\sum_{i=1}^p E((u_i - d_i)^2 | X_i) \right)$$

$$= \frac{p\tau^2}{1+\tau^2} + (p-2)^2 / [(p-2)(1+\tau^2)]$$

$$= \frac{2(p-2)}{1+\tau^2} + ((1+\tau^2) \cdot p) / (1+\tau^2)^2$$

$$= \frac{p\tau^2}{1+\tau^2} + \frac{p-2}{1+\tau^2} - \frac{2(p-2)}{1+\tau^2} + \frac{p(1+\tau^2)}{1+\tau^2}$$

$$= \frac{p\tau^2 + p-2 - 2p+4 + p}{1+\tau^2} = \frac{p\tau^2 + 2}{1+\tau^2}$$